# baseURI: http://www.w3.org/ns/dcat
    # imports: http://purl.org/dc/terms/
    # imports: http://www.w3.org/2004/02/skos/core
    # imports: http://www.w3.org/ns/prov-o#
    # prefix: usg

@prefix dcat:  <http://www.w3.org/ns/dcat#> .
@prefix dcterms:   <http://purl.org/dc/terms/> .
@prefix dctype: <http://purl.org/dc/dcmitype/> .
@prefix foaf:  <http://xmlns.com/foaf/0.1/#> .
@prefix owl:   <http://www.w3.org/2002/07/owl#> .
@prefix prov:  <http://www.w3.org/ns/prov#> .
@prefix rdf:   <http://www.w3.org/1999/02/22-rdf-syntax-ns#> .
@prefix rdfs:  <http://www.w3.org/2000/01/rdf-schema#> .
@prefix sdo:   <http://schema.org/#> .
@prefix skos:  <http://www.w3.org/2004/02/skos/core#> .
@prefix vcard: <http://www.w3.org/2006/vcard/ns#> .
@prefix xsd:   <http://www.w3.org/2001/XMLSchema#> .
@prefix usg:   <http://resources.data.gov/resources/dcat-us/#> .
@prefix sh:    <http://www.w3.org/ns/shacl#> .

<http://resources.data.gov/resources/dcat-us/#>
    a owl:Ontology ;
    dcterms:contributor [
        sdo:affiliation [
            foaf:homepage <http://dhs.gov> ;
        foaf:name "U.S. Department of Homeland Security" ;
        ] ;
    foaf:name "Simson Garfinkel" ;
    ] ;
    dcterms:modified "2021-10-20"^^xsd:date ;
    rdfs:comment "DCAT extensions in DCAT-US and further extended by DHS";
    owl:imports dcterms: ;
    owl:imports <http://www.w3.org/2004/02/skos/core> ;
    owl:imports <http://www.w3.org/ns/prov-o#> ;
    owl:versionInfo "Initial Version";
    .

usg:accessLevel
    a rdf:Property ;
    a sh:NodeShape ;

    rdfs:range rdfs:Literal ;
    rdfs:label "Access Level"@en ;
    rdfs:isDefinedBy <https://resources.data.gov/resources/dcat-us/> ;
    rdfs:comment "The degree to which this dataset could be made publicly-available, regardless of whether it has been made available. Choices: public (Data asset is or could be made publicly available to all without restrictions), restricted public (Data asset is available under certain use restrictions), or non-public (Data asset is not available to members of the public)." ;

    sh:property [
        sh:in ( usg:public usg:restrictedPublic  usg:nonPublic ) ;
    ] ;
    .

usg:systemOfRecords
    a rdf:Property ;
    rdfs:label "System of Records"@en ;
    rdfs:isDefinedBy <https://resources.data.gov/resources/dcat-us/> ;
    rdfs:range rdfs:Literal ;
    rdfs:comment "The system of records notice (SORN) in which the dataset appears." ;
    .

usg:describedBy
    a rdf:Property ;
    rdfs:label "Described By"@en ;
    rdfs:isDefinedBy <http://resources.data.gov/resources/dcat-us/> ;
    rdfs:range rdfs:Literal ;
    rdfs:comment "URL for the JSON Schema file that defines the schema used." ;
    .

usg:describedByType
    a rdf:Property ;
    rdfs:label "Described By Type"@en ;
    rdfs:isDefinedBy <http://resources.data.gov/resources/dcat-us/> ;
    rdfs:range rdfs:Literal ;
    rdfs:comment "The machine-readable file format (IANA Media Type also known as MIME Type) of the dataset's Data Dictionary (describedBy)." ;
    .

usg:dataQuality
    a rdf:Property ;
    rdfs:label "Data Quality"@en ;
    rdfs:isDefinedBy <http://resources.data.gov/resources/dcat-us/> ;
    rdfs:range rdfs:Literal ;
    rdfs:comment "Indicates whether a dataset conforms to the agency's information quality guidelines (boolean)." ;
    .

usg:modified
    a rdf:Property ;
    rdfs:label "Modified"@en ;
    rdfs:isDefinedBy <http://resources.data.gov/resources/dcat-us/> ;
    rdfs:range rdfs:Literal ;
    rdfs:comment "Most recent date on which the dataset was changed, updated or modified." ;
    .

usg:public
    a rdfs:Property ;
    rdfs:label "public"@en ;
    rdfs:comment "Data asset is or could be made publicly available to all without restrictions." ;
    .

usg:restrictedPublic
    a owl:DatatypeProperty ;
    rdfs:label "restricted public"@en ;
    rdfs:comment "A restricted public dataset is one only available under certain conditions or to certain audiences (such as researchers who sign a waiver)." ;
    .

usg:nonPublic
    a owl:DatatypeProperty ;
    rdfs:label "non-public"@en ;
    rdfs:comment "A non-public dataset is one that could never be made available to the public for privacy, security, or other reasons as determined by your agency." ;
    .

usg:primaryITInvestmentUII
    a rdf:Property ;
    rdfs:label "Primary IT Investment UII"@en ;
    rdfs:isDefinedBy <http://resources.data.gov/resources/dcat-us/> ;
    rdfs:range rdfs:Literal ;
    rdfs:comment "For linking a dataset with an IT Unique Investment Identifier (UII). Can have multiple comma separated values." ;
    .